\documentclass[12pt]{article}
\usepackage[utf8]{inputenc}
\usepackage[
a4paper,		% papel A4
left=2cm,		% margem esquerda
right=2cm,		% margem direita
top=2cm,		% margem superior
bottom=2cm		% margem inferior
]{geometry}
\usepackage[T1]{fontenc}
\usepackage{array,latexsym,amssymb}
\usepackage{amsmath,amsfonts,amssymb,amsthm,mathabx,amstext}
\usepackage{dsfont}	% Conjuntos: $\mathds{N, Z, Q, R, C}$
\usepackage{graphicx}
\begin{document}
\begin{center}
	UNIVERSIDADE FEDERAL DA PARAÍBA\\
	Probabilidade II\\
	Atividade 4\\
	Paulo Ricardo Seganfredo Campana
\end{center}

\noindent Questão 1.\\

$X\sim Exp\left(\lambda = \dfrac{1}{10}\right)\qquad\qquad F_{X}(x)=1-e^{-\dfrac{x}{10}}$\\

\noindent a) $P(X>10)=1-P(X\leq10)=1-F_{X}(10)$\\

$1-(1-e^{-1})=1-1+e^{-1}=\dfrac{1}{e}$\\

\noindent b) $P(10\leq X\leq20)=F_{X}(20)-F_{X}(10)$\\

$(1-e^{-2})-(1-e^{-1})=e^{-1}-e^{-2}=\dfrac{1}{e}-\dfrac{1}{e^{2}}$\\

\noindent Questão 2.\\

\noindent a) $S_{Y}=Y\circ S_{x}=h(X)\circ(0,1)=(0,\infty)$\\

\noindent b) $X\sim U(0,1)\longrightarrow F_{X}(x)=x$\\

$F_{Y}(y)=P(Y\leq y)=P(-\ln(1-X)\leq y)=P(\ln(1-X)\geq -y)=P(1-X\geq e^{-y})$\\

$P(-X\geq e^{-y}-1)=P(X\leq1-e^{-y})=F_{X}(1-e^{-y})=1-e^{-y}$\\

$F_{Y}(y)=\left\{\begin{array}{@{}l@{}}0\text{,\qquad\quad se }y<0,\\1-e^{-y}\text{, se }y\geq0.\end{array}\right.$\\

\noindent c) $F_{Y}'(y)=e^{-y}$\\

$f_{Y}(y)=\left\{\begin{array}{@{}l@{}}0\text{,\hspace{+11pt} se }y<0,\\e^{-y}\text{, se }y\geq0.\end{array}\right.\longrightarrow Y\sim Exp(\lambda = 1)$\\

\noindent Questão 3.\\

$M_{X}(t)=E(e^{xt})=\displaystyle\int_{0}^{\infty}e^{tx}\lambda e^{-\lambda x}dx=\displaystyle\int_{0}^{\infty}\lambda e^{-(\lambda-t)x}dx\hfill u=(\lambda-t)x\quad du=(\lambda-t)dx$\\

$\dfrac{\lambda}{\lambda-t}\displaystyle\int_{0}^{\infty}e^{-u}du=\dfrac{\lambda}{\lambda-t}$\\

$M_{X}'(t)=\dfrac{\lambda}{(\lambda-t)^{2}}\longrightarrow M_{X}'(0)=\dfrac{\lambda}{\lambda^{2}}=\dfrac{1}{\lambda}$\\

$M_{X}''(t)=\dfrac{2\lambda}{(\lambda-t)^{3}}\longrightarrow M_{X}''(0)=\dfrac{2\lambda}{\lambda^{3}}=\dfrac{2}{\lambda^{2}}\hfill\dfrac{2}{\lambda^{2}}-\left(\dfrac{1}{\lambda}\right)^{2}=\dfrac{1}{\lambda^{2}}$\\

$E(X)=\dfrac{1}{\lambda},\qquad Var(X)=\dfrac{1}{\lambda^{2}}$\\

\noindent Questão 4.\\

$\displaystyle\int_{-2}^{2}cdx+\int_{2}^{4}2cdx=1\longrightarrow cx\biggr|^{2}_{-2}+2cx\biggr|^{4}_{2}=1\longrightarrow(2c+2c)+(8c-4c)=1\longrightarrow8c=1\longrightarrow c=\dfrac{1}{8}$\\

$E(X)=\dfrac{1}{8}\left(\displaystyle\int_{-2}^{2}xdx+\int_{4}^{2}2xdx\right)=\dfrac{1}{8}\left(\dfrac{x^{2}}{2}\biggr|^{2}_{-2}+x^{2}\biggr|^{4}_{2}\right)=\dfrac{1}{8}\left(2-2+16-4\right)=\dfrac{12}{8}=\dfrac{3}{2}$\\

$E(X^{2})=\dfrac{1}{8}\left(\displaystyle\int_{-2}^{2}x^{2}dx+\int_{4}^{2}2x^{2}dx\right)=\dfrac{1}{8}\left(\dfrac{x^{3}}{3}\biggr|^{2}_{-2}+\dfrac{2x^{3}}{3}\biggr|^{4}_{2}\right)=\dfrac{1}{24}\left(8+8+128-16\right)=\dfrac{16}{3}$\\

$E(X)=\dfrac{3}{2},\qquad Var(X)=\dfrac{16}{3}-\left(\dfrac{3}{2}\right)^{2}=\dfrac{37}{12}$\\

\noindent Questão 5.\\

\noindent a) $E(Y)=E(-\ln X)\qquad f_{Y}=1\cdot\mathds{I}_{(0,1)}(x)$\\

$\displaystyle\int_{-\infty}^{\infty}-\ln x\cdot\mathds{I}_{(0,1)}(x)dx=\int_{0}^{1}-\ln xdx=\int_{1}^{0}\ln xdx$\\

$x\ln x-x\biggr|_{1}^{0}=(0\cdot(-\infty)-0)-(1\cdot\ln 1-1)=1$\\

\noindent b) $X\sim U(0,1)\longrightarrow F_{X}(x)=x$\\

$F_{Y}(y)=P(Y\leq y)=P(-\ln X\leq y)=P(\ln X\geq -y)=P(X\geq e^{-y})$\\

$1-P(X\leq e^{-y})=1-F_{X}(e^{-y})=1-e^{-y}$\\

$f_{Y}(y)=F_{Y}'(y)=e^{-y}\longrightarrow Y\sim Exp(\lambda=1)$\\

\noindent c) $S_{Y}=(0,\infty)$\\

$E(Y)=\displaystyle\int_{0}^{\infty}ye^{-y}dy\hfill\left\{\begin{array}{@{}l@{}}u=y,\qquad du=dy\\v=-e^{-y},\quad dv=e^{-y}\end{array}\right.$\\

$\displaystyle -ye^{-y}\biggr|^{\infty}_{0}+\int_{0}^{\infty}e^{-y}dy\longrightarrow-\dfrac{y}{e^{y}}\biggr|^{\infty}_{0}+1\longrightarrow E(Y)=1$\\

Alternativamente:\\

$E\left(Y\sim Exp\left(\lambda\right)\right) = \dfrac{1}{\lambda}\longrightarrow\lambda=1\longrightarrow E(Y)=1\quad\checkmark$\\












\end{document}